april-asp/src/asp.lean
@@ -1,0 +1,126 @@
+import order.hom.complete_lattice
+import program
+import order.fixed_points
+open tv
+open order_hom
+
+#check order_hom.lfp
+
+
+def xT_propagate (i_pos i_neg : I) : Program -> I
+| [] := i_pos
+| (r::p) := (i_pos.assign r.head (r.eval_body i_pos i_neg)) ⊔ (xT_propagate p)
+
+def T_propagate (p : Program) (i_neg i_pos : I) : I := xT_propagate i_pos i_neg p
+
+
+theorem T_monotone (p : Program) (i_neg : I) : monotone (T_propagate p i_neg) := λ a b c, begin
+  induction p,
+  exact c,
+  refine sup_le_sup _ p_ih,
+  refine I.assign_step c _,
+  exact Rule.eval_body_monotone p_hd i_neg c,
+end
+
+def T (p : Program) (i_neg : I) : I →o I := ⟨T_propagate p i_neg, T_monotone p i_neg⟩
+
+
+lemma T_increasing {p : Program} {i ii : I} : ii <= T p i ii := begin
+  induction p, refl,
+  exact le_sup_of_le_right p_ih,
+end
+
+
+@[simp] lemma  T_fp_le_eq_iff {p : Program} {i ii : I} : T p i ii <= ii ↔ T p i ii = ii := 
+  (iff.intro (λ h, le_antisymm h T_increasing) (λ h, (eq.symm h).ge))
+
+lemma T_fp_eq_unstep {p_tl : Program} {p_hd : Rule}  {i ii : I} (h : i = T (p_hd::p_tl) ii i) : i = T p_tl ii i  := 
+  le_antisymm T_increasing (sup_le_iff.mp (le_antisymm_iff.mp h).right).right
+
+lemma T_fp_rule_sat_iff {p : Program} {i ii : I} : i = T p ii i ↔ ∀ r ∈ p, Rule.reduct_satisfied r i ii := begin
+  -- ==>
+  split; assume h,
+  induction p,
+  by_contradiction, finish,
+  assume r rmem,
+  change r.eval_body i ii <= r.eval_head i,
+  cases rmem, rw <- rmem at h,
+  change i = (λ b, if r.head = b then (r.eval_body i ii) else i b) ⊔ (xT_propagate i ii p_tl) at h,  
+  cases r.eval_body i ii,
+  any_goals { rw h, unfold Rule.eval_head, refine le_sup_iff.mpr _, left, simp },
+  exact p_ih (T_fp_eq_unstep h) r rmem,
+  -- <==
+  refine le_antisymm T_increasing _,
+  induction p, 
+  exact rfl.ge,
+  change (i.assign p_hd.head (p_hd.eval_body i ii)) ⊔ (xT_propagate i ii p_tl) <= i,
+  apply sup_le_iff.mpr,
+  split,
+  have h2 := @h p_hd (or.inl rfl), change p_hd.eval_body i ii <= p_hd.eval_head i at h2,
+  unfold I.assign,
+  refine I.less_than_or_equal.mk _, assume a,
+  split_ifs,
+  rw <- h_1, exact h2,
+  exact rfl.le,
+  refine p_ih _, simp at *, assume r rmem, exact h.right r rmem,
+end
+
+theorem T_fp_model_iff {p : Program} {i : I} : i = T p i i ↔ p.model i :=
+  (iff.intro (λ h, ⟨ T_fp_rule_sat_iff.mp h ⟩)
+             (λ h, T_fp_rule_sat_iff.mpr h.p))
+
+
+
+
+
+lemma fuck {p : Program} {i ii : I} (k : i = Inf {a : I | (T p ii) a ≤ a}) : (T p ii) i = i := begin
+  refine funext _, assume a,
+
+end
+
+#check lfp
+
+
+theorem T_fp_stable_model_iff {p : Program} {i : I}: i = lfp (T p i) ↔ p.stable_model i := begin
+split; assume h,
+unfold lfp at h, simp at h,
+change i = Inf {a : I | (T p i) a = a} at h,
+have i_fp : (T p i) i = i := begin
+  -- suggest,
+end,
+refine Program.stable_model.mk (T_fp_model_iff.mp h) _,
+sorry,
+
+-- all_goals { assume h },
+-- unfold_coes, unfold lfp, simp, unfold_coes, unfold T, simp,
+-- by_contradiction u,
+-- let jj := i ⊓ Inf {a : I | T_propagate p i a ≤ a},
+-- let j : jj < i := sorry,
+-- have pp := h.p jj j,
+
+
+
+-- exact sorry,
+-- -- simp,
+-- refine Inf_le_of_le _ _,
+-- assume b bm,
+
+-- exact sorry,
+-- exact Inf_le (T_model_fp' model),
+
+-- -- by_contradiction q, simp at q,
+-- -- simp at q,
+-- exact sorry,
+-- -- Eliminate the Inf :)
+-- -- simp,
+-- assume b tp,
+
+
+-- exact sorry,
+-- fconstructor, assumption,
+-- assume ii ii_lt_i,
+-- by_contradiction,
+-- have u := h.p,
+-- have uy := model.p,
+-- sorry
+end
