april-asp/src/program.lean
@@ -1,0 +1,298 @@
+/-
+Defines a normal ASP program and its three-valued semantics
+-/
+
+import primitives
+open tv
+open order_hom
+open atom
+
+structure Rule :=
+  (head : atom)
+  (pbody : list atom)
+  (nbody : list atom)
+def Program := list Rule
+
+
+set_option trace.simplify.rewrite true
+
+#check Inf_eq_bot
+
+namespace Rule
+  def eval_pbody (self : Rule) (i : I) : tv := tv.conj (i.eval self.pbody) 
+  def eval_nbody (self : Rule) (i : I) : tv := tv.conj (tv.negl (i.eval self.nbody))
+  def eval_body (self : Rule) (i_pos i_neg : I) : tv := (self.eval_pbody i_pos) ⊓ (self.eval_nbody i_neg)
+  def eval_head (self : Rule) (i : I) : tv := i self.head
+
+  @[simp] def eval_pbody_monotone (r : Rule) : monotone r.eval_pbody := λ a b c, begin
+    unfold Rule.eval_pbody,
+    induction r.pbody, exact rfl.ge,
+    unfold tv.conj at |- ih, unfold tv.inf at |- ih,
+    rw [I.unfold_eval a, I.unfold_eval b],
+    have t : ⊤ = vtrue := by { refl },
+    have rd_a := tv.foldl_remove_default (a hd),
+    have rd_b := tv.foldl_remove_default (b hd),
+    rw t at rd_a rd_b, rw [rd_a, rd_b], rw [@tv.foldl_min_extract (a hd), @tv.foldl_min_extract (b hd)],
+    exact min_le_min (c.p hd) ih,
+  end
+
+  def eval_body_monotone (r : Rule) (i_neg : I) : monotone (λ i_pos, r.eval_body i_pos i_neg) :=
+      λ a b c, inf_le_inf (eval_pbody_monotone r c) (rfl.ge)
+
+  def reduct_satisfied (r : Rule) (i_pos i_neg : I) : Prop := r.eval_body i_pos i_neg <= r.eval_head i_pos
+  def satisfied (r : Rule) (i : I) := r.reduct_satisfied i i
+end Rule
+
+instance : has_mem Rule Program := ⟨@list.mem Rule⟩ 
+namespace Program
+  structure reduct_model (self : Program) (i_pos i_neg : I) : Prop :=
+    (p : ∀r ∈ self, Rule.reduct_satisfied r i_pos i_neg)
+  def model (self : Program) (i : I) := self.reduct_model i i
+  structure stable_model (self : Program) (i : I) : Prop :=
+    (m : self.model i)
+    (p : ∀ii < i, ¬(self.reduct_model ii i))
+
+  def atoms (p : Program) : set atom := {
+    a : atom | ∃ (r : Rule) (m : r ∈ p), a = r.head ∨ a ∈ r.pbody ∨ a ∈ r.nbody
+  }
+
+  def atoms_list : Program -> list atom
+  | [] := []
+  | (r::tl) := (r.head::(r.pbody ++ r.nbody)) ++ (atoms_list tl)
+
+lemma atoms_atoms_list_mem_iff {p : Program} (a : atom) : a ∈ p.atoms ↔ a ∈ p.atoms_list := begin     split; assume h,     induction p,      cases h, cases h_h, change false at h_h_w,     contradiction,     cases h with r h2, cases h2 with r_mem acond,     cases r_mem,     unfold atoms_list,     cases acond,     rw [<-r_mem, acond],     exact list.mem_cons_self r.head ((r.pbody ++ r.nbody).append (atoms_list p_tl)),     cases acond; right; rw <-r_mem,     change a ∈ ((r.pbody ++ r.nbody) ++ (atoms_list p_tl)),     rw list.mem_append_eq, left, rw list.mem_append_eq, left,     exact acond,     change a ∈ ((r.pbody ++ r.nbody) ++ (atoms_list p_tl)),     rw list.mem_append_eq, left, rw list.mem_append_eq, right,     exact acond, right,     change a ∈ ((p_hd.pbody ++ p_hd.nbody) ++ (atoms_list p_tl)),     change r ∈ p_tl at r_mem,     rw list.mem_append_eq, right,     refine p_ih _,     exact Exists.intro r (Exists.intro r_mem acond),     induction p, change false at h, contradiction,     cases h,     refine Exists.intro p_hd (Exists.intro (list.mem_cons_self p_hd p_tl) _),     exact or.inl h,     change a ∈ ((p_hd.pbody ++ p_hd.nbody) ++ (atoms_list p_tl)) at h,     repeat {rw list.mem_append_eq at h},     repeat {cases h},     refine Exists.intro p_hd (Exists.intro (list.mem_cons_self p_hd p_tl) _),     right, left, exact h,     refine Exists.intro p_hd (Exists.intro (list.mem_cons_self p_hd p_tl) _),     right, right, exact h,     have h2 := p_ih h,     cases h2 with r h3, cases h3 with rmem acond,     have rmem2 : r ∈ p_hd :: p_tl := list.mem_of_mem_tail rmem,     exact Exists.intro r (Exists.intro rmem2 acond),   end 
+
+instance program_atom_mem_decidable {p : Program} {a : atom} : decidable (a ∈ p.atoms) := begin
+  rw (@atoms_atoms_list_mem_iff p a),
+  exact @list.decidable_mem atom atom.decidable_eq a p.atoms_list
+end 
+
+  -- An interpretation bound to a program p
+  @[ext]
+  structure I (p : Program) :=
+    (e : Π (a : atom) (m : a ∈ p.atoms), tv)
+
+
+end Program
+
+def Program.localize (p : Program) (i : I) : p.I := ⟨λ a amem, i a⟩ 
+def Program.I.i {p : Program} (pi : p.I) : I := λ a, (dite (a ∈ p.atoms)
+  (λ c, pi.e a c)
+  (λ a, vfalse))
+
+
+
+
+
+
+namespace Program
+  @[simp] lemma I_eq_PI {p : Program} (pi : p.I) : (p.localize (pi.i)) = pi := begin
+    ext a amem,
+    change dite (a ∈ p.atoms) (λ (c : a ∈ p.atoms), pi.e a c) (λ (a : a ∉ p.atoms), vfalse) = pi.e a amem,
+    split_ifs, refl,
+  end
+  lemma I.i.inj {p : Program} : function.injective (@Program.I.i p) := begin
+    assume pi1 pi2 pii_eq,
+    ext a amem,
+    rw [<-I_eq_PI pi1, <-I_eq_PI pi2, pii_eq],
+  end
+end Program
+
+instance {p : Program} : has_coe p.I I := ⟨Program.I.i⟩
+def Program.I.sup {p : Program} (a b : p.I) : p.I := p.localize $ I.sup a b
+instance {p : Program} : has_sup p.I := ⟨@Program.I.sup p⟩
+def Program.I.inf {p : Program} (a b : p.I) : p.I := p.localize $ I.inf a b
+instance {p : Program} : has_inf p.I := ⟨@Program.I.inf p⟩
+def Program.I.bot {p : Program} := p.localize I.bot
+instance {p : Program} : has_bot p.I := ⟨@Program.I.bot p⟩
+def Program.I.top {p : Program} := p.localize I.top
+instance {p : Program} : has_top p.I := ⟨@Program.I.top p⟩
+instance Program.I.partial_order {p : Program} : partial_order p.I := partial_order.lift (@Program.I.i p) (@Program.I.i.inj p)
+
+def Program.I.less_than_or_equal (p : Program) := (@Program.I.partial_order p).le
+
+variable p : Program
+#check (@Program.I.partial_order p).le
+
+lemma Program.I.bot_eq_I_bot {p : Program} : (@Program.I.bot p).i = I.bot := by {ext, unfold Program.I.i, split_ifs; refl}
+
+lemma Program.I.le_top {p : Program} (pi : p.I) : pi <= ⊤ := begin
+  change pi.i <= Program.I.top.i,
+  apply I.less_than_or_equal.mk, assume a,
+  unfold Program.I.i, split_ifs,
+  exact le_top, exact rfl.le,
+end
+lemma Program.I.bot_le {p : Program} (pi : p.I) : ⊥ <= pi := begin
+  change Program.I.bot.i <= pi,
+  rw Program.I.bot_eq_I_bot,
+  exact bot_le,
+end
+
+instance Program.I.bounded_order {p : Program} : bounded_order p.I := {
+  top := Program.I.top,
+  le_top := Program.I.le_top,
+  bot := Program.I.bot,
+  bot_le := Program.I.bot_le,
+}
+
+
+@[simp] lemma Program.I.sup_distrib {p : Program} (a b : p.I) : (a ⊔ b).i = a.i ⊔ b.i := begin
+  ext, change (a ⊔ b).i x = (a.i ⊔ b.i) x,
+  change dite (x ∈ p.atoms) (λ (c : x ∈ p.atoms), (a ⊔ b).e x c) (λ (a : x ∉ p.atoms), vfalse) = (a.i ⊔ b.i) x,
+  split_ifs,
+  change (p.localize $ I.sup a.i b.i).e x h = (a.i ⊔ b.i) x,
+  unfold Program.localize, simp, refl,
+  change vfalse = if (b.i x) <= (a.i x) then (a.i x) else (b.i x),
+  split_ifs,
+  all_goals { unfold Program.I.i; finish },
+end
+
+@[simp] lemma Program.I.inf_distrib {p : Program} (a b : p.I) : (a ⊓ b).i = a.i ⊓ b.i := begin
+  ext, change (a ⊓ b).i x = (a.i ⊓ b.i) x,
+  change dite (x ∈ p.atoms) (λ (c : x ∈ p.atoms), (a ⊓ b).e x c) (λ (a : x ∉ p.atoms), vfalse) = (a.i ⊓ b.i) x,
+  split_ifs,
+  change (p.localize $ I.inf a.i b.i).e x h = (a.i ⊓ b.i) x,
+  unfold Program.localize, simp, refl,
+  change vfalse = min (a.i x) (b.i x),
+  change vfalse = if (a.i x) <= (b.i x) then (a.i x) else (b.i x),
+  split_ifs,
+  all_goals { unfold Program.I.i; finish },
+end
+
+
+
+-- These wrapper proofs are longer than the original proofs :(
+@[simp] lemma Program.I.sup_le {p : Program} (a b c : p.I) : a <= c -> b <= c -> a ⊔ b <= c := begin
+  change a.i ≤ c.i → b.i ≤ c.i → (p.localize (a.i ⊔ b.i)).i ≤ c.i,
+  rw [<-Program.I.sup_distrib, Program.I_eq_PI, Program.I.sup_distrib],
+  exact I.sup_le a b c,
+end
+@[simp] lemma Program.I.le_sup_right {p : Program} (a b : p.I) : b <= a ⊔ b := begin
+  change b.i <= (p.localize (a.i ⊔ b.i)).i,
+  rw [<-Program.I.sup_distrib, Program.I_eq_PI, Program.I.sup_distrib],
+  exact I.le_sup_right a b,
+end
+@[simp] lemma Program.I.le_sup_left {p : Program} (a b : p.I) : a <= a ⊔ b := begin
+  change a.i <= (p.localize (a.i ⊔ b.i)).i,
+  rw [<-Program.I.sup_distrib, Program.I_eq_PI, Program.I.sup_distrib],
+  exact I.le_sup_left a b,
+end
+@[simp] lemma Program.I.le_inf {p : Program} (a b c : p.I) : a <= b -> a <= c -> a <= b ⊓ c := begin
+  change a.i ≤ b.i → a.i ≤ c.i → a.i <= (p.localize (b.i ⊓ c.i)).i,
+  rw [<-Program.I.inf_distrib, Program.I_eq_PI, Program.I.inf_distrib],
+  exact I.le_inf a b c,
+end
+@[simp] lemma Program.I.inf_le_right {p : Program} (a b : p.I) : a ⊓ b <= b:= begin
+  change (p.localize (a.i ⊓ b.i)).i <= b.i,
+  rw [<-Program.I.inf_distrib, Program.I_eq_PI, Program.I.inf_distrib],
+  exact I.inf_le_right a b,
+end
+@[simp] lemma Program.I.inf_le_left {p : Program} (a b : p.I) : a ⊓ b <= a := begin
+  change (p.localize (a.i ⊓ b.i)).i <= a.i,
+  rw [<-Program.I.inf_distrib, Program.I_eq_PI, Program.I.inf_distrib],
+  exact I.inf_le_left a b,
+end
+
+
+instance {p : Program} : has_coe (set p.I) (set I) := ⟨set.image Program.I.i⟩
+
+@[reducible] 
+noncomputable def Program.I.Sup {p : Program} (S : set p.I) : p.I := p.localize $ I.Sup S
+@[reducible] 
+noncomputable instance Program.I.has_Sup {p : Program} : has_Sup p.I := ⟨@Program.I.Sup p⟩
+@[reducible]
+noncomputable def Program.I.Inf {p : Program} (S : set p.I) : p.I := p.localize $ I.Inf S
+@[reducible] 
+noncomputable instance Program.I.has_Inf {p : Program} : has_Inf p.I := ⟨@Program.I.Inf p⟩
+
+
+@[simp] lemma Program.I.Sup_distrib {p : Program} (S : set p.I) : (Program.I.Sup S).i = I.Sup (Program.I.i '' S) := begin
+  ext, change dite (x ∈ p.atoms) (λ (c : x ∈ p.atoms), (Program.I.Sup S).e x c) (λ (a : x ∉ p.atoms), vfalse) = I.Sup (Program.I.i '' S) x,
+  split_ifs, refl,
+  change vfalse = tv.Sup ((λ (i : I), i x) '' (Program.I.i '' S)),
+  symmetry, apply Sup_eq_bot.mpr, assume a b,
+  simp at b, cases b with z x, rw <-x.right, unfold Program.I.i, simp, split_ifs, refl,
+end
+
+-- Unlike Program.I.Sup_distrib, this only works when S is nonempty
+@[simp] lemma Program.I.Inf_distrib {p : Program} {S : set p.I} (Snm : S.nonempty) : (Program.I.Inf S).i = I.Inf (Program.I.i '' S) := begin
+  ext, change dite (x ∈ p.atoms) (λ (c : x ∈ p.atoms), (Program.I.Inf S).e x c) (λ (a : x ∉ p.atoms), vfalse) = I.Inf (Program.I.i '' S) x,
+  split_ifs, refl,
+  change vfalse = tv.Inf ((λ (i : I), i x) '' (Program.I.i '' S)),
+  symmetry, apply Inf_eq_bot.mpr, assume a b,
+  simp at b, refine Exists.intro ⊥ (Exists.intro _ _), work_on_goal 2 { exact b,},
+  simp, cases Snm with y1 y2, refine Exists.intro y1 (and.intro y2 _),
+  unfold Program.I.i, simp, finish,
+end
+
+
+
+lemma Program.I.le_Sup {p : Program} (S : set p.I) (i : p.I) (m : i ∈ S) : i <= (Program.I.Sup S) := begin
+  change i.i <= (p.localize $ I.Sup (Program.I.i '' S)).i,
+  rw [<-Program.I.Sup_distrib, Program.I_eq_PI, Program.I.Sup_distrib],
+  exact I.le_Sup S i (set.mem_image_of_mem (Program.I.i) m),
+end
+-- Too tired for this lol
+lemma Program.I.Sup_le {p : Program} (S : set p.I) (i : p.I) (pp : ∀ o ∈ S, o <= i) : (Program.I.Sup S) <= i := begin
+  have h := I.Sup_le S i (λ o omem, begin
+    -- have hh := 
+    have g := pp (p.localize o),
+    have t : p.localize o ∈ S := begin
+      sorry
+    end,
+    have gg := g t,
+    change (p.localize o).i ≤ i.i at gg,
+    change o <= i.i,
+  end),
+  change (p.localize $ I.Sup (Program.I.i '' S)).i <= i.i,
+  rw [<-Program.I.Sup_distrib, Program.I_eq_PI, Program.I.Sup_distrib],
+  exact h,
+end
+lemma Program.I.Inf_le {p : Program} (S : set p.I) (i : p.I) (m : i ∈ S) : (I.Inf S) <= i := sorry
+lemma Program.I.le_Inf {p : Program} (S : set p.I) (i : p.I) (pp : ∀ o ∈ S, i <= o) : i <= (Program.I.Inf S) := sorry
+
+#check set.mem_image_of_mem
+
+-- We can't use function.injective.lattice to lift the lattice from I because Program.I.i destroys info in the interpretation
+
+
+#check partial_order.lift (@Program.I.i p) (@Program.I.i.inj p)
+
+  -- @[reducible] noncomputable instance complete_lattice : complete_lattice I := {
+  --   le := I.le,
+  --   sup := I.sup,
+  --   sup_le := I.sup_le,
+  --   le_sup_right := I.le_sup_right,
+  --   le_sup_left := I.le_sup_left,
+  --   inf := I.inf,
+  --   le_inf := I.le_inf,
+  --   inf_le_right := I.inf_le_right,
+  --   inf_le_left := I.inf_le_left,
+  --   Sup := I.Sup,
+  --   le_Sup := I.le_Sup,
+  --   Sup_le := I.Sup_le,
+  --   Inf := I.Inf,
+  --   le_Inf := I.le_Inf,
+  --   Inf_le := I.Inf_le,
+  --   ..I.partial_order,
+  --   ..I.bounded_order,
+  -- }
+
+
+#check distrib
+
+#check (@Program.I.i.inj p).lattice
+#check function.injective.lattice (@Program.I.i p) (@Program.I.i.inj p) (λ a b, begin
+  change (p.localize $ I.sup a b).i = a.i ⊔ b.i,
+  unfold_coes,
+  -- rw Program.I_eq_PI (a.i.sup b.i),
+  --  rw [<-Program.I_eq_PI a, <-Program.I_eq_PI b],
+   
+  -- ext,
+  -- unfold Program.I.i, split_ifs,  
+end) 
+instance {p : Program} : lattice p.I := 
+
+
+
+#check le_sup_iff.mpr
